ReadMe.md
@@ -6,4 +6,33 @@ Currently what is formalized is:
 
 - Normalization-By-Eval for Monoid-rewriting (Slides 25-35)
 
-- Normalization-By-Eval for Godel's system T (slides 62-70)
+- Normalization-By-Eval for Godel's system T (Slides 62-70)
+
+
+# Build instructions for Verso-textbook
+To build the Verso-textbook documenting the code:
+
+1. Run `lake exe cache get`: 
+    
+    This makes it so mathlib is quick to build
+
+2. Run `lake build`:
+
+    This builds the `.lake` directory.
+
+3. Copy the code from `_in/textbook/DemoTextbook.lean` and paste it all into `.lake/packages/verso/examples/textbook/DemoTextbook.lean`:
+
+    This is an ugly work-around I did, since I didn't know how to deal with git-submodules (verso is a submodule of my git-repo) and because the .lake directory is git-ignored.
+Because of both of these things, I did the easiest workaround for myself: I manually copied the code from  `.lake/packages/verso/examples/textbook/DemoTextbook.lean` and put it in the unused `_in/textbook/DemoTextbook.lean` so git could keep track of my verso-code.
+When you build verso in the `lake build` step, it is going to have the example code from the verso-repo. So in this step you are manually replacing the example-code with the verso-code I have written.
+
+4. Run `lake exe demotextbook --output _out/examples/demotextbook`:
+
+    This will take the verso code from `.lake/packages/verso/examples/textbook/DemoTextbook.lean`, build the textbook from it, and put everything in the `_out` directory.
+
+5. Run `python3 -m http.server 8880 --directory _out/examples/demotextbook/html-single &`:
+
+    This creates a local server where you can read the textbook that was built.
+
+6. View the textbook in your browser with `http://localhost:8880/`
+
